coq/TestDesign3/UntypedProperties/CommonProperties.v
@@ -1,0 +1,54 @@
+(*! Properties that are useful to reason about untyped semantics !*)
+(* TODO: move this to the kôika repo *)
+Require Export Koika.Utils.Common.
+Require Import Koika.KoikaForm.Untyped.UntypedSemantics.
+Require Import Koika.KoikaForm.SimpleVal.
+Require Import Koika.KoikaForm.Untyped.UntypedLogs.
+
+Section Logs.
+    Context {V: Type}.
+
+    Context {reg_t: Type}.
+    Context {REnv: Env reg_t}.
+    Definition R : reg_t -> Type := fun _ => V.
+
+    Notation Log := (@_ULog V reg_t REnv).
+
+    Lemma log_find_empty {T} idx (f: @LogEntry (R idx) -> option T):
+        log_find (log_empty: Log) idx f = None.
+    Proof.
+        unfold log_find, log_empty; intros; rewrite getenv_create; reflexivity.
+    Qed.
+
+    Lemma log_app_assoc : forall (l1 l2 l3: Log),
+        log_app (log_app l1 l2) l3 = log_app l1 (log_app l2 l3).
+    Proof.
+        unfold log_app, map2; intros.
+        apply create_funext. intros.
+        rewrite !getenv_create.
+        rewrite app_assoc.
+        reflexivity.
+    Qed.
+
+    Lemma log_app_empty_l : forall (l: Log),
+        log_app log_empty l = l.
+    Proof.
+        intros.
+        apply equiv_eq.
+        unfold equiv, log_app, map2, log_empty; intros.
+        rewrite !getenv_create, app_nil_l.
+        reflexivity.
+    Qed.
+
+    Lemma log_app_empty_r : forall (l: Log),
+        log_app l log_empty = l.
+    Proof.
+        intros.
+        apply equiv_eq.
+        unfold equiv, log_app, map2, log_empty; intros.
+        rewrite !getenv_create, app_nil_r.
+        reflexivity.
+    Qed.
+
+
+End Logs.
